\section*{Problem 2}

Prove that when
\[0 \to A^\bullet \to B^\bullet \to C^\bullet \to 0\]
is a s.e.s of cohomological complexes in degree \(\ge 0\),
we have the associated long exact sequence of the cohomology modules.

\subsection*{Proof}

Use Snake Lemma.

First, for each integer \(k\), we have,
\[\begin{tikzcd}
  0 \ar{r} & A^k \ar["f^k"]{d} \ar{r} & B^k \ar["g^k"]{d} \ar{r} & C^k \ar["h^k"]{d} \ar{r} & 0 \\
  0 \ar{r} & A^{k+1} \ar{r} & B^{k+1} \ar{r} & C^{k+1} \ar{r} & 0
  \end{tikzcd}\]
By Snake Lemma, we obtain the below exact sequence:
\[\begin{tikzcd}
  0 \ar{r}
  & \ker f^k \ar{r}
  & \ker g^k \ar{r}
  & \ker h^k \ar["\partial"]{r}
  & \coker f^k \ar{r}
  & \coker g^k \ar{r}
  & \coker h^k \ar{r}
  & 0
  \end{tikzcd}\]
Note that \(\coker f^k = A^{k + 1} / \im f^k\).

In this case, we can define
\(\tilde f^k: A^k / \im f^{k - 1} \to \ker f^{k + 1}\)
as
\(\tilde f^k(x + \im f^{k-1}) = f^k(x)\).
It's well-defined because,
if \(x + \im f^{k-1} = y + \im f^{k-1}\),
\(x - y \in \im f^{k-1} \subseteq \ker f^k\)
thus \(f^k(x - y) = 0\)
and \(f^k(x) = f^k(x) - f^k(x - y) = f^k(x - x + y) = f^k(y)\).
Also, because \(\im f^k \subseteq \ker f^{k + 1}\), the image of \(\tilde f^k\) is in \(\ker f^{k+1}\).

Then, we have:
\[\begin{tikzcd}
  & \coker f^{k-1} \ar["\tilde f^k"]{d} \ar{r} & \coker g^{k-1} \ar["\tilde g^k"]{d} \ar{r} & \coker h^{k-1} \ar["\tilde h^k"]{d} \ar{r} & 0 \\
  0 \ar{r} & \ker f^{k + 1} \ar{r} & \ker g^{k + 1} \ar{r} & \ker h^{k + 1} &
  \end{tikzcd}\]
and each rows of above diagram are exact because of the result of Snake Lemma.

Suppose that \(\tilde f^k(x + \im f^{k-1}) = 0\).
Then, \(x \in \ker f^k\), and \(x + \im f^{k-1} \in \ker f^k / \im f^{k-1}\).
The converse is also true,
because \(x + \im f^{k-1} \in \ker f^k / \im f^{k-1}\)
implies \(x \in \ker f^k\) and \(\tilde f^k(x + \im f^{k-1}) = f^k(x) = 0\).
Thus, \(\ker \tilde f^k = \ker f^k / \im f^{k - 1} = H^k(A^\bullet)\).

Also, \(\coker \tilde f^k = \cod(\tilde f^k) / \im \tilde f^k = \ker f^{k+1} / \im f^k = H^{k + 1}(A^\bullet)\).

In the same way, we can show that
\(H^k(B^\bullet) = \ker\tilde g^k = \coker\tilde g^{k - 1}\),
\(H^k(C^\bullet) = \ker\tilde h^k = \coker\tilde h^{k - 1}\).

Thus, by Snake Lemma,
\[\begin{tikzcd}
  H^k(A^\bullet) \ar{r}
  & H^k(B^\bullet) \ar{r}
  & H^k(C^\bullet) \ar["\partial"]{r}
  & H^{k+1}(A^\bullet) \ar{r}
  & H^{k+1}(B^\bullet) \ar{r}
  & H^{k+1}(C^\bullet)
  \end{tikzcd}\]
Repeating this for every integer \(k\), we obtain:
\[\begin{tikzcd}
  \cdots \ar{r}
  & H^{k - 1}(C^\bullet) \ar{r}
  & H^k(A^\bullet) \ar{r}
  & H^k(B^\bullet) \ar{r}
  & H^k(C^\bullet) \ar{r}
  & H^{k+1}(A^\bullet) \ar{r}
  & \cdots
  \end{tikzcd}\]
\qedsq

Note: \(\partial\) is defined as below (the proof is in HW5 Problem 7)
Let \(x \in \ker\coker h^{k-1} = \im\coker g^{k-1}\).
Then, there is \(x'\) which is mapped to \(x\) by \(\coker g^{k-1} \to \coker h^{k-1}\).
Then, let \(y'\) be an image of \(x'\) into \(\ker g^{k+1}\).
Then, let \(y \in \ker f^{k+1}\) which is mapped to \(y'\) in \(\ker g^{k+1}\).
\(\partial(x) = y + \im (\coker f^{k-1} \to \ker f^{k+1})\).