\section*{Problem 3}

Give a rigorous proof of the below theorem:

\begin{theorem}
(Pseudo-universal property)
Let \(M, N\) be \(R\)-modules, and let \(f^{-1}: M \to N\) be a \(R\)-module homomorphism.
Let \(M \to E^\bullet\) and \(N \to I^\bullet\) be injective resolutions.
Then there is a chain map \(f^\bullet : E^\bullet \to I^\bullet\)
that extends \(f^{-1}\).
Furthermore, this \(f^\bullet\) is unique up to chain homotopy.
\end{theorem}

\subsection*{Proof}

The below diagram shows the ingrediants given in the problem.
Dashed arrows are what we should construct.

\[\begin{tikzcd}
  0 \ar{r} & M \ar["f^{-1}"]{d} \ar["g^{-1}"]{r} & E^0 \ar[dashed, "f^0"]{d} \ar["g^0"]{r} & E^1 \ar[dashed, "f^1"]{d} \ar{r} & \cdots \\
  0 \ar{r} & N \ar["h^{-1}"]{r} & I^0 \ar["h^0"]{r} & I^1 \ar{r} & \cdots
\end{tikzcd}\]

We'll denote \(E^{-1} = M\), \(I^{-1} = N\), \(E^{-2} = I^{-2} = 0\), \(g^{-2}: 0 \to M, h^{-2}: 0 \to N\) are zero functions.

\subsubsection*{Existence of \(f^\bullet\)}

Suppose that we already have \(f^{-1}, \cdots, f^{k}\) for some \(k \in \bbZ^{\ge -1}\),
such that \(f^{j + 1} g^{j} = h^{j} f^j\) for every \(j \in \{-1, 0, \cdots, k - 1\}\) (i.e. they commute as the above diagram).

Then, we can make induced homomorphisms
\(\tilde g^{k}: \coker g^{k - 1} = E^{k} / \im g^{k - 1} \to E^{k + 1}\) such that \(\tilde g^{k}(x + \im g^{k - 1}) = g^{k}(x)\),
\(\tilde h^{k}: \coker h^{k - 1} = I^{k} / \im h^{k - 1} \to I^{k + 1}\) such that \(\tilde h^{k}(x + \im h^{k - 1}) = h^{k}(x)\),
and
\(\tilde f^{k}: \coker g^{k - 1} \to \coker h^{k - 1}\) such that
\(\tilde f^{k}(x + \im g^{k - 1}) = f^{k}(x) + \im h^{k - 1}\).

Note that above isomorphisms are well defined
Because
if \(x + \im g^{k - 1} = y + \im g^{k - 1}\),
then \(x - y \in \im g^{k - 1} = \ker g^{k}\),
and \(g^{k}(x) - g^{k}(y) = g^{k}(x - y) = 0\).
In the same way, \(\tilde h^{k}\) is well-defined.
If \(x + \im g^{k - 1} = y + \im g^{k - 1}\),
\(x - y \in \im g^{k - 1}\).
Let \(t \in E^{k - 1}\) such that \(g^{k - 1}(t) = x - y\).
\(f^k(x - y) = h^{k - 1}(f^{k - 1}(t))\).
Thus, \(f^k(x - y) \in \im h^{k - 1}\).
This shows \(\tilde f^k\) is well-defined.

\(\tilde g^{k}\) is injective.
Because \(\ker g^{k} = \im g^{k - 1}\) because of exactness of seqneuce,
if \(x + \im g^{k - 1} \in \ker \tilde g^{k}\),
\(g^{k}(x) = \tilde g^{k}(x + \im g^{k - 1}) = 0\)
and
\(x \in \ker g^{k} = \im g^{k - 1}\).
But in this case, \(x + \im g^{k - 1} = \im g^{k - 1}\),
which is an additive identity of \(\coker g^{k - 1}\).
This shows that \(\ker \tilde g^{k}\) contains only an additive identity
and \(\tilde g^{k}\) is injective.
In the same way, we can show that \(\tilde h^{k}\) is also injective.

Then, rows of the below diagram are exact.
\[\begin{tikzcd}
  0 \ar{r} & \coker g^{k - 1} \ar["\tilde f^{k}"]{d} \ar["\tilde g^{k}"]{r} & E^{k + 1} \ar[dashed, "f^{k + 1}"]{d} \ar{r} & \cdots \\
  0 \ar{r} & \coker h^{k - 1} \ar["\tilde h^{k}"]{r} & I^{k + 1} \ar{r} & \cdots
\end{tikzcd}\]

Since \(\tilde g^{k - 1}\) is injective,
by injectivity of \(I^{k + 1}\),
we can extend \(\tilde h^k \circ \tilde f^k\) to \(f^{k + 1}: E^{k + 1} \to I^{k + 1}\).
Then, because \(f^{k + 1}\) is an extension,
\(\tilde h_{k} \circ \tilde f^{k} = f^{k + 1} \circ \tilde g_{k}\).

Lastly, let's check \(h_{k} \circ f^{k} = f^{k + 1} \circ g_{k}\).
Note that
\(g^{k - 1}(x) = \tilde g^{k - 1}(x + \im g^{k})\)
and
\(h^{k - 1}(x) = \tilde h^{k - 1}(x + \im h^{k})\).
In other words,
\((f^{k + 1} \circ \tilde g^{k})(x + \im g^{k}) = (f^{k + 1} \circ g^{k})(x)\)
,
\((\tilde h^{k} \circ \tilde f^{k})(x + \im g^{k}) = \tilde h^{k}(f^{k}(x) + \im h^{k}) = (h^{k} \circ f^{k})(x)\)
thus,
\[(h^{k} \circ f^{k})(x) = (\tilde h^{k} \circ \tilde f^{k})(x + \im g^{k}) =
  (f^{k + 1} \circ \tilde g^{k})(x + \im g^{k}) = (f^{k + 1} \circ g^{k})(x) \]
Therefore, \(h^{k} \circ f^{k} = f^{k + 1} \circ g^{k}\).

The above process constructs \(f^{k + 1}\) from \(f^{k}\) such that
\(h^{k} \circ f^{k} = f^{k + 1} \circ g^{k}\) holds.
Because \(f^{-1}\) was given,
we can construct \(f^\bullet\) by repeating above process.
\qedsq

%-------------------------------------------------------------------------------

\subsubsection*{Uniqueness of \(f^\bullet\)}

Suppose that there are two extensions \(f^\bullet\) and \(f'^\bullet\) from \(f\).
Let \(\varphi^\bullet = f^\bullet - f'^\bullet\).
Note that \(\varphi^{-1}\) is a zero map.

\[\begin{tikzcd}
  0 \ar{r} & M \ar[swap, "\varphi^{-1} = 0"]{d} \ar["g^{-1}"]{r} & E^0 \ar["\varphi^{0}"]{d} \ar["g^{0}"]{r} \ar[dashed, "s^0"]{ld} & E^1 \ar{r} \ar[dashed, "s^1"]{ld} & \cdots \\
  0 \ar{r} & N \ar[swap,"h^{-1}"]{r} & I^0 \ar{r} &  \cdots
\end{tikzcd}\]

If we find \(s^\bullet: E^{\bullet} \to I^{\bullet - 1}\) such that
\(\varphi^k = s^{k + 1} g^k + h^k s^k\), \(f\) and \(f'\) are chain homotopy equivalence by \(s\).

First, let \(\cdots, s^{-2}, s^{-1}\) are zero maps.

Let \(s^{0} = 0\).
Then, \(0 = \varphi^{-1} = h^{-2}s^{-1} + s^{0}g^{-1} = 0 + 0 = 0\) holds.

Suppose that for \(k \in \bbN\), for every integer \(n < k\),
\(\varphi^{n} = h^{n - 1}s^{n} + s^{n + 1}g^{n}\) holds.

Let \(\psi^{k} = \varphi^k - h^{k - 1}s^{k}\)

Let \(x \in \ker g^k = \im g^{k - 1}\). Then, there is \(y \in E^{k - 1}\) such that \(g^{k - 1}(y) = x\). Then, because \(h^{k - 1} \circ h^{k - 2} = 0\),
\begin{align*}
  \psi^k (x)
  = (\varphi^k - h^{k - 1}s^{k}) (x)
  &= (\varphi^k g^{k - 1} - h^{k - 1}s^{k}g^{k - 1}) (y)
  \\&= ( h^{k - 1} \varphi^{k - 1} - h^{k - 1}s^{k}g^{k - 1}) (y)
  \\&= ( h^{k - 1}(h^{k - 2}s^{k - 1} + s^{k}g^{k - 1}) - h^{k - 1}s^{k}g^{k - 1}) (y)
  \\&= ( h^{k - 1}h^{k - 2}s^{k - 1} + h^{k - 1}s^{k}g^{k - 1} - h^{k - 1}s^{k}g^{k - 1}) (y)
  \\&= ( h^{k - 1}h^{k - 2}s^{k - 1}) (y)
  \\&= ( 0 \circ s^{k - 1}) (y) = 0
\end{align*}

Therefore, \(\ker g^k \subseteq \ker \psi^k\).

In this case, if \(x + \im g^{k - 1}, y + \im g^{k - 1} \in \coker g^{k - 1}\) satisfies
\(x + \im g^{k - 1} = y + \im g^{k - 1}\),
\(x - y \in \im g^{k - 1} = \ker g^k\) and \(\psi^k(x - y) = 0\).
Therefore, if we make an induced homomorphism \(\tilde \psi^k: \coker g^{k - 1} \to I^k\)
such that \(\tilde \psi^{k}(x + \im g^{k - 1}) = \psi^k(x)\),
it's well-defined.

Also, note that we showed that there is
an induced injective homomorphism \(\tilde g^{k - 1}: \coker g^{k - 1} \to E^{k + 1}\)
in the proof of ``Existence of \(f^\bullet\)''.

\[\begin{tikzcd}
  0 \ar{r} & \coker g^{k - 1} \ar[swap, "\tilde \psi^k"]{d} \ar["\tilde g^{k}"]{r} & E^{k + 1} \ar[dashed, "s^{k + 1}"]{ld} \\
  & I^{k} & 
\end{tikzcd}\]

Therefore, by injectivity of \(I^k\),
we can extend \(\tilde \psi^{k}\) to \(s^{k + 1}\) such that \(\tilde \psi^{k} = s^{k + 1} \circ \tilde g^{k}\).

Let's check \(\psi^k = s^{k + 1} \circ g^k\).
Because \(\psi^k(x) = \tilde \psi^k(x + \im g^{k - 1})\) and \(g^k(x) = \tilde g^k(x + \im g^{k - 1})\), for any \(x \in E^k\),
\[\psi^k(x) = \tilde\psi^k(x + \im g^{k - 1}) = s^{k + 1}(\tilde g^k(x + \im g^{k - 1})) = s^{k + 1}(g^k(x))\].

Therefore, we obtained \(s^{k + 1}\) such that
\[\psi^k = \varphi^k - h^{k - 1}s^k = s^{k + 1}g^k\]

Then, by induction, we can find \(s^\bullet\) which satisfies above equation.
In other words, for every \(k \in \bbZ^{\ge 0}\),
\[f^k - f'^k = \varphi^k = h^{k - 1}s^k + s^{k + 1}g^k\]
holds.
Thus, we can construct a chain homotopy for two extensions \(f^\bullet\) and \(f'^\bullet\) which extended from \(f^{-1}\).

Therefore, \(f^k\) are unique up to chain homotopy.
\qedsq